add # special case to npbc_check

examples/pseudo_bool/npbc_checkScript.sml
@@ -726,9 +726,16 @@ Definition mem_constraint_def:
     if equal_constraint c x then T else mem_constraint c xs
 End
 
+(* Checking triviality for a negated target c *)
+Definition check_triv_def:
+  check_triv extra nc =
+  (check_contradiction (add extra nc) ∨
+  check_contradiction nc)
+End
+
 (* Partition the formula goals into proved and non-proved
   For each non-proved goal, check if
-  0) it is implied by extra (= ¬ C)
+  0) it is implied by extra (= ¬ C) or trivial
   1) it was already in the formula
   2) it was already proved by another proofgoal (excluding #)
 *)
@@ -740,7 +747,7 @@ Definition split_goals_def:
     PARTITION (λ(i,c). sptree$lookup i proved ≠ NONE) goals in
   let proved = MAP SND lp in
   let f = range fml in
-  EVERY (λ(i,c). c ∈ f ∨ imp extra c ∨ mem_constraint c proved) lf
+  EVERY (λ(i,c). c ∈ f ∨ check_triv extra (not c) ∨ mem_constraint c proved) lf
 End
 
 Triviality list_pair_eq_thm:
@@ -776,6 +783,11 @@ Definition mk_subst_def:
   (mk_subst xs = INR (spt_to_vec (fromAList xs)))
 End
 
+Definition check_hash_triv_def:
+  check_hash_triv extra ncs =
+    EXISTS (check_triv extra) ncs
+End
+
 (* The tcb flag indicates we're in to-core mode
   where it is guaranteed that the core formula implies derived *)
 Definition check_red_def:
@@ -798,8 +810,11 @@ Definition check_red_def:
           let goals = toAList (map_opt (subst_opt w) gfml) in
           let (l,r) = extract_pids pfs LN LN in
             split_goals gfml nc l goals ∧
-            EVERY (λid. lookup id r ≠ NONE)
-              (COUNT_LIST (LENGTH rsubs)))
+            EVERY (λ(id,cs).
+              lookup id r ≠ NONE ∨
+              check_hash_triv nc cs
+              )
+              (enumerate 0 rsubs))
         | SOME cid =>
           check_contradiction_fml b fml' cid) in
       if chk then
@@ -1062,7 +1077,7 @@ QED
 Theorem split_goals_checked:
   split_goals fml e proved goals ∧
   MEM (n,yy) goals ⇒
-  yy ∈ range fml ∨ imp e yy ∨
+  yy ∈ range fml ∨ check_triv e (not yy) ∨
   ∃i.
     lookup i proved ≠ NONE ∧
     MEM (i,yy) goals
@@ -1164,6 +1179,53 @@ Proof
   gvs[AllCaseEqs()]
 QED
 
+Theorem MEM_enumerate_index:
+  ∀k xs.
+  MEM (i,e) (enumerate k xs) ⇒
+  ∃j. j < LENGTH xs ∧ i = k + j
+Proof
+  Induct_on`xs`>>rw[miscTheory.enumerate_def]
+  >- intLib.ARITH_TAC>>
+  first_x_assum drule>>
+  rw[]
+  >- intLib.ARITH_TAC
+QED
+
+Theorem MEM_enumerate_iff:
+  MEM ie (enumerate 0 xs) ⇔
+  ∃i e. ie = (i,e) ∧ i < LENGTH xs ∧ EL i xs = e
+Proof
+  Cases_on`ie`>>
+  rename1`MEM (i,e) _ `>>
+  Cases_on`i < LENGTH xs`>>fs[MEM_enumerate]
+  >- metis_tac[]>>
+  CCONTR_TAC>>fs[]>>
+  drule MEM_enumerate_index>>
+  rw[]
+QED
+
+Theorem check_triv_unsatisfiable:
+  check_triv extra nc ⇒
+  unsatisfiable (fml ∪ {extra} ∪ {nc})
+Proof
+  rw[check_triv_def]>>
+  drule check_contradiction_unsat>>
+  rw[unsatisfiable_def,satisfiable_def]>>
+  metis_tac[add_thm]
+QED
+
+Theorem check_triv_unsatisfiable_2:
+  check_triv extra nc ∧
+  extra ∈ fml ∧ nc ∈ fml
+  ⇒
+  unsatisfiable fml
+Proof
+  rw[check_triv_def]>>
+  drule check_contradiction_unsat>>
+  rw[unsatisfiable_def,satisfiable_def,satisfies_def]>>
+  metis_tac[add_thm]
+QED
+
 Theorem check_red_correct:
   id_ok fml id ∧
   OPTION_ALL good_spo ord ∧
@@ -1224,55 +1286,89 @@ Proof
   \\ drule sat_implies_transitive
   \\ disch_then (fn th => DEP_REWRITE_TAC[th])
   \\ simp [Once implies_explode]
-  \\ gvs[red_subgoals_def,MEM_COUNT_LIST,ADD1]
+  \\ gvs[red_subgoals_def,MEM_enumerate_iff,ADD1,AND_IMP_INTRO,PULL_EXISTS]
   \\ reverse (rw [])
   >- (
     (* dominance *)
     rw[sat_implies_EL]>>
-    last_x_assum(qspec_then`SUC n` assume_tac)>>
+    last_x_assum(qspec_then`SUC n` mp_tac)>>
     gvs[]>>
-    drule_all lookup_extract_pids_r>> rw[]
-    \\ drule extract_clauses_MEM_INR
-    \\ disch_then drule
-    \\ fs[EL]
-    \\ DEP_REWRITE_TAC [EL_APPEND_EQN] \\ simp[]
-    \\ rw[]
-    \\ first_x_assum drule \\ strip_tac
-    \\ gs[EL_MAP]
-    \\ drule unsatisfiable_not_sat_implies
-    \\ simp[range_insert]
-    \\ metis_tac[INSERT_SING_UNION,UNION_COMM])
+    PURE_REWRITE_TAC[METIS_PROVE [] ``((P ⇒ Q) ⇒ R) ⇔ (~P ∨ Q) ⇒ R``]>>
+    strip_tac
+    >- (
+      drule_all lookup_extract_pids_r>> rw[]
+      \\ drule extract_clauses_MEM_INR
+      \\ disch_then drule
+      \\ fs[EL]
+      \\ DEP_REWRITE_TAC [EL_APPEND_EQN] \\ simp[]
+      \\ rw[]
+      \\ first_x_assum drule \\ strip_tac
+      \\ gs[EL_MAP]
+      \\ drule unsatisfiable_not_sat_implies
+      \\ simp[range_insert]
+      \\ metis_tac[INSERT_SING_UNION,UNION_COMM])
+   >- (
+      fs[check_hash_triv_def]
+      \\ pop_assum mp_tac
+      \\ DEP_REWRITE_TAC [EL_APPEND_EQN]
+      \\ simp[EL_MAP]
+      \\ strip_tac
+      \\ match_mp_tac unsatisfiable_not_sat_implies
+      \\ metis_tac[check_triv_unsatisfiable]) )
   >- (
     (* objective *)
-    Cases_on`obj`>>
-    last_x_assum(qspec_then`SUC(LENGTH (dom_subst (subst_fun (mk_subst s)) ord))` assume_tac)>>
-    fs[]>>
-    drule_all lookup_extract_pids_r>>rw[]
-    \\ drule extract_clauses_MEM_INR
-    \\ disch_then drule
-    \\ fs[EL]
-    \\ DEP_REWRITE_TAC [EL_APPEND2]
-    \\ simp[]
-    \\ rw[]
-    \\ first_x_assum drule \\ strip_tac
-    \\ gs[]
-    \\ drule unsatisfiable_not_sat_implies
-    \\ simp[range_insert]
-    \\ metis_tac[INSERT_SING_UNION,UNION_COMM])
+    Cases_on`obj`>> gvs[]>>
+    last_x_assum(qspec_then`SUC(LENGTH (dom_subst (subst_fun (mk_subst s)) ord))` mp_tac)>>
+    gvs[]>>
+    PURE_REWRITE_TAC[METIS_PROVE [] ``((P ⇒ Q) ⇒ R) ⇔ (~P ∨ Q) ⇒ R``]>>
+    strip_tac
+    >- (
+      drule_all lookup_extract_pids_r>>rw[]
+      \\ drule extract_clauses_MEM_INR
+      \\ disch_then drule
+      \\ fs[EL]
+      \\ DEP_REWRITE_TAC [EL_APPEND2]
+      \\ simp[]
+      \\ rw[]
+      \\ first_x_assum drule \\ strip_tac
+      \\ gs[]
+      \\ drule unsatisfiable_not_sat_implies
+      \\ simp[range_insert]
+      \\ metis_tac[INSERT_SING_UNION,UNION_COMM])
+    >- (
+      fs[check_hash_triv_def]
+      \\ pop_assum mp_tac
+      \\ DEP_REWRITE_TAC [EL_APPEND_EQN]
+      \\ simp[EL_MAP]
+      \\ strip_tac
+      \\ match_mp_tac unsatisfiable_not_sat_implies
+      \\ metis_tac[check_triv_unsatisfiable])
+    )
   >- (
     (* redundancy #0 *)
-    last_x_assum(qspec_then`0` assume_tac)>>
-    fs[]>>
-    drule_all lookup_extract_pids_r>>rw[]
-    \\ drule extract_clauses_MEM_INR
-    \\ disch_then drule
-    \\ fs[]
-    \\ rw[]
-    \\ first_x_assum drule \\ strip_tac
-    \\ fs[]
-    \\ drule unsatisfiable_not_sat_implies
-    \\ simp[range_insert]
-    \\ metis_tac[INSERT_SING_UNION,UNION_COMM])
+    last_x_assum(qspec_then`0` mp_tac)>>
+    gvs[]>>
+    PURE_REWRITE_TAC[METIS_PROVE [] ``((P ⇒ Q) ⇒ R) ⇔ (~P ∨ Q) ⇒ R``]>>
+    strip_tac
+    >- (
+      drule_all lookup_extract_pids_r>>rw[]
+      \\ drule extract_clauses_MEM_INR
+      \\ disch_then drule
+      \\ fs[]
+      \\ rw[]
+      \\ first_x_assum drule \\ strip_tac
+      \\ fs[]
+      \\ drule unsatisfiable_not_sat_implies
+      \\ simp[range_insert]
+      \\ metis_tac[INSERT_SING_UNION,UNION_COMM])
+    >- (
+      fs[check_hash_triv_def]
+      \\ pop_assum mp_tac
+      \\ DEP_REWRITE_TAC [EL_APPEND_EQN]
+      \\ simp[EL_MAP]
+      \\ strip_tac
+      \\ match_mp_tac unsatisfiable_not_sat_implies
+      \\ metis_tac[check_triv_unsatisfiable]))
   (* rest of redundancy *)
   \\ gvs [GSYM unsat_iff_implies]
   \\ Cases_on ‘subst_opt (subst_fun (mk_subst s)) x'’ \\ fs []
@@ -1297,7 +1393,8 @@ Proof
     simp[]>>
     metis_tac[range_mk_core_fml,in_core_only_fml_or_left])
   >- (
-    fs[satisfiable_def,not_thm,satisfies_def]>>
+    drule check_triv_unsatisfiable>>
+    fs[unsatisfiable_def,satisfiable_def,not_thm,satisfies_def]>>
     drule subst_opt_SOME >>
     metis_tac[not_thm,imp_thm,in_core_only_fml_or_left])
   \\ drule_all lookup_extract_pids_l>>rw[]
@@ -1770,7 +1867,11 @@ Definition check_reflexivity_def:
   (case check_subproofs cpfs F fml id of
     SOME (fml',id') =>
     let (l,r) = extract_pids pfs LN LN in
-       EVERY (λid. lookup id r ≠ NONE) (COUNT_LIST (LENGTH dsubs))
+       EVERY (λ(id,cs).
+              lookup id r ≠ NONE ∨
+              EXISTS check_contradiction cs
+              )
+              (enumerate 0 dsubs)
   | _ => F)
 End
 
@@ -1786,7 +1887,12 @@ Definition check_transitivity_def:
   (case check_subproofs cpfs F fml id of
     SOME (fml',id') =>
     let (l,r) = extract_pids pfs LN LN in
-    if EVERY (λid. lookup id r ≠ NONE) (COUNT_LIST (LENGTH dsubs))
+    if
+       EVERY (λ(id,cs).
+              lookup id r ≠ NONE ∨
+              EXISTS check_contradiction cs
+              )
+              (enumerate 0 dsubs)
     then SOME id'
     else NONE
   | _ => NONE)
@@ -1931,8 +2037,12 @@ Definition check_change_obj_def:
         NONE => NONE
       | SOME (fml',id') =>
         let (l,r) = extract_pids pfs LN LN in
-        if EVERY (λid. lookup id r ≠ NONE)
-             (COUNT_LIST (LENGTH csubs))
+        if
+          EVERY (λ(id,cs).
+              lookup id r ≠ NONE ∨
+              EXISTS check_contradiction cs
+              )
+              (enumerate 0 csubs)
         then
           SOME (fc',id')
         else NONE))
@@ -2014,8 +2124,11 @@ Definition check_cstep_def:
             let (l,r) = extract_pids pfs LN LN in
             let gfml = mk_core_fml F fml in
               split_goals gfml nc l goals ∧
-              EVERY (λid. lookup id r ≠ NONE)
-                (COUNT_LIST (LENGTH dsubs))
+              EVERY (λ(id,cs).
+                lookup id r ≠ NONE ∨
+                check_hash_triv nc cs
+              )
+              (enumerate 0 dsubs)
           | SOME cid =>
             check_contradiction_fml F fml' cid) in
         if check then
@@ -2400,7 +2513,7 @@ Proof
       `pc.id ∉ domain fml` by fs[id_ok_def]>>
       fs[core_only_fml_F_insert_b]>>
       fs[EVERY_MEM,MEM_MAP,EXISTS_PROD]>>
-      gvs[dom_subgoals_def,MEM_COUNT_LIST,ADD1]>>
+      gvs[dom_subgoals_def,MEM_enumerate_iff,ADD1,AND_IMP_INTRO,PULL_EXISTS]>>
       CONJ_TAC >- (
         (* core constraints*)
         rw[sat_implies_def,satisfies_def]
@@ -2423,10 +2536,13 @@ Proof
           drule subst_opt_SOME >>
           rw[]>> metis_tac[not_thm])
         >- (
-          fs[satisfiable_def,not_thm,satisfies_def]>>
+          drule check_triv_unsatisfiable>>
+          disch_then(qspec_then`{}` mp_tac)>>
+          fs[unsatisfiable_def,satisfiable_def,not_thm,satisfies_def]>>
           drule subst_opt_SOME >>
           fs[range_def]>>
-          rw[]>> metis_tac[not_thm,imp_thm])
+          rw[]>>
+          metis_tac[not_thm,imp_thm])
         \\ drule_all lookup_extract_pids_l>>rw[]
         \\ drule_all extract_clauses_MEM_INL
         \\ strip_tac
@@ -2453,29 +2569,75 @@ Proof
         fs[core_only_fml_def]>>
         simp[GSYM LIST_TO_SET_MAP]>>
         rw[sat_implies_EL,EL_MAP]>>
-        last_x_assum(qspec_then`n` assume_tac)>>
+        last_x_assum(qspec_then`n` mp_tac)>>
         gvs[dom_subst_def]>>
-        drule_all lookup_extract_pids_r>>
-        rw[]>>
-        drule extract_clauses_MEM_INR>>
-        disch_then drule>>
-        fs[EL_MAP]>>
-        DEP_REWRITE_TAC [EL_APPEND_EQN] >> simp[]>>
-        simp[EL_MAP]>>
-        rw[]>>
-        first_x_assum drule >> strip_tac>>
-        gs[]>>
-        drule unsatisfiable_not_sat_implies>>
-        simp[lookup_list_list_insert,ALOOKUP_ZIP_MAP]>>
-        simp[range_insert]>>
-        metis_tac[INSERT_SING_UNION,UNION_COMM])>>
+        PURE_REWRITE_TAC[METIS_PROVE [] ``((P ⇒ Q) ⇒ R) ⇔ (~P ∨ Q) ⇒ R``]>>
+        strip_tac
+        >- (
+          drule_all lookup_extract_pids_r>>
+          rw[]>>
+          drule extract_clauses_MEM_INR>>
+          disch_then drule>>
+          fs[EL_MAP]>>
+          DEP_REWRITE_TAC [EL_APPEND_EQN] >> simp[]>>
+          simp[EL_MAP]>>
+          rw[]>>
+          first_x_assum drule >> strip_tac>>
+          gs[]>>
+          drule unsatisfiable_not_sat_implies>>
+          simp[lookup_list_list_insert,ALOOKUP_ZIP_MAP]>>
+          simp[range_insert]>>
+          metis_tac[INSERT_SING_UNION,UNION_COMM])
+        >- (
+          fs[check_hash_triv_def]
+          \\ pop_assum mp_tac
+          \\ DEP_REWRITE_TAC [EL_APPEND_EQN]
+          \\ simp[EL_MAP]
+          \\ simp[lookup_list_list_insert,ALOOKUP_ZIP_MAP]
+          \\ strip_tac
+          \\ match_mp_tac unsatisfiable_not_sat_implies
+          \\ metis_tac[check_triv_unsatisfiable])
+      )>>
       CONJ_TAC >- (
         (* negated order constraint *)
         fs[core_only_fml_def]>>
-        last_x_assum(qspec_then`LENGTH (dom_subst (subst_fun (mk_subst l)) (SOME ((x0,x1,x2),x3)))` assume_tac)>>
+        last_x_assum(qspec_then`LENGTH (dom_subst (subst_fun (mk_subst l)) (SOME ((x0,x1,x2),x3)))` mp_tac)>>
         gs[ADD1]>>
+        PURE_REWRITE_TAC[METIS_PROVE [] ``((P ⇒ Q) ⇒ R) ⇔ (~P ∨ Q) ⇒ R``]>>
+        strip_tac
+        >- (
+          drule_all lookup_extract_pids_r>>
+          simp[]>> rw[]
+          \\ drule extract_clauses_MEM_INR
+          \\ disch_then drule
+          \\ fs[]
+          \\ DEP_REWRITE_TAC [EL_APPEND2]
+          \\ simp[]
+          \\ rw[]
+          \\ first_x_assum drule \\ strip_tac
+          \\ gs[neg_dom_subst_def,lookup_list_list_insert,ALOOKUP_ZIP_MAP,range_insert]
+          \\ metis_tac[INSERT_SING_UNION,UNION_COMM,LIST_TO_SET_MAP])
+        >- (
+          fs[check_hash_triv_def]
+          \\ pop_assum mp_tac
+          \\ DEP_REWRITE_TAC [EL_APPEND_EQN]
+          \\ gs[neg_dom_subst_def,lookup_list_list_insert,ALOOKUP_ZIP_MAP,range_insert,EXISTS_MEM,MEM_MAP]
+          \\ strip_tac \\ rw[]
+          \\ drule check_triv_unsatisfiable_2
+          \\ disch_then match_mp_tac
+          \\ simp[])
+        )>>
+      (* objective constraint *)
+      fs[core_only_fml_def]>>
+      Cases_on`pc.obj`>>
+      simp[]>>
+      last_x_assum(qspec_then`SUC(LENGTH (dom_subst (subst_fun (mk_subst l)) (SOME ((x0,x1,x2),x3))))` mp_tac)>>
+      gs[ADD1]>>
+      PURE_REWRITE_TAC[METIS_PROVE [] ``((P ⇒ Q) ⇒ R) ⇔ (~P ∨ Q) ⇒ R``]>>
+      strip_tac
+      >- (
         drule_all lookup_extract_pids_r>>
-        simp[]>> rw[]
+        simp[]>>rw[]
         \\ drule extract_clauses_MEM_INR
         \\ disch_then drule
         \\ fs[]
@@ -2483,26 +2645,19 @@ Proof
         \\ simp[]
         \\ rw[]
         \\ first_x_assum drule \\ strip_tac
-        \\ gs[neg_dom_subst_def,lookup_list_list_insert,ALOOKUP_ZIP_MAP,range_insert]
-        \\ metis_tac[INSERT_SING_UNION,UNION_COMM,LIST_TO_SET_MAP])>>
-      (* objective constraint *)
-      fs[core_only_fml_def]>>
-      Cases_on`pc.obj`>>
-      simp[]>>
-      last_x_assum(qspec_then`SUC(LENGTH (dom_subst (subst_fun (mk_subst l)) (SOME ((x0,x1,x2),x3))))` assume_tac)>>
-      gs[ADD1]>>
-      drule_all lookup_extract_pids_r>>
-      simp[]>>rw[]
-      \\ drule extract_clauses_MEM_INR
-      \\ disch_then drule
-      \\ fs[]
-      \\ DEP_REWRITE_TAC [EL_APPEND2]
-      \\ simp[]
-      \\ rw[]
-      \\ first_x_assum drule \\ strip_tac
-      \\ gs[range_insert]
-      \\ drule unsatisfiable_not_sat_implies
-      \\ metis_tac[INSERT_SING_UNION,UNION_COMM])>>
+        \\ gs[range_insert]
+        \\ drule unsatisfiable_not_sat_implies
+        \\ metis_tac[INSERT_SING_UNION,UNION_COMM])
+      >- (
+          fs[check_hash_triv_def]
+          \\ pop_assum mp_tac
+          \\ DEP_REWRITE_TAC [EL_APPEND_EQN]
+          \\ simp[EL_MAP]
+          \\ simp[lookup_list_list_insert,ALOOKUP_ZIP_MAP]
+          \\ strip_tac
+          \\ match_mp_tac unsatisfiable_not_sat_implies
+          \\ metis_tac[check_triv_unsatisfiable])
+      )>>
     CONJ_TAC >- (
       pop_assum mp_tac>>
       DEP_REWRITE_TAC[core_only_fml_F_insert_b]>>
@@ -2724,22 +2879,33 @@ Proof
       rw[]>>
       simp[GSYM LIST_TO_SET_MAP]>>
       rw[sat_implies_EL]>>
-      fs[EVERY_MEM,MEM_COUNT_LIST]>>
+      fs[EVERY_MEM,MEM_enumerate_iff,PULL_EXISTS]>>
       first_x_assum drule>>
-      rw[]>>
-      drule_all lookup_extract_pids_r>>
-      simp[]>>
-      rw[]>>
-      drule extract_clauses_MEM_INR>>
-      disch_then drule>>
-      simp[EL_MAP]>>
-      rw[]>>
-      first_x_assum drule>>
-      simp[]>>rw[]>>
-      drule unsatisfiable_not_sat_implies>>
-      simp[core_only_fml_def,Abbr`fmll`] >>
-      once_rewrite_tac [subst_eta] >> fs [] >>
-      gvs [ALOOKUP_APPEND,ALOOKUP_ZIP_MAP])>>
+      PURE_REWRITE_TAC[METIS_PROVE [] ``((P ⇒ Q) ⇒ R) ⇔ (~P ∨ Q) ⇒ R``]>>
+      strip_tac
+      >- (
+        drule_all lookup_extract_pids_r>>
+        simp[]>>
+        rw[]>>
+        drule extract_clauses_MEM_INR>>
+        disch_then drule>>
+        simp[EL_MAP]>>
+        rw[]>>
+        first_x_assum drule>>
+        simp[]>>rw[]>>
+        drule unsatisfiable_not_sat_implies>>
+        simp[core_only_fml_def,Abbr`fmll`] >>
+        once_rewrite_tac [subst_eta] >> fs [] >>
+        gvs [ALOOKUP_APPEND,ALOOKUP_ZIP_MAP])
+      >- (
+        gvs[EL_MAP]>>
+        match_mp_tac unsatisfiable_not_sat_implies>>
+        simp[]>>
+        drule check_contradiction_unsat>>
+        simp[unsatisfiable_def,satisfiable_def]>>
+        once_rewrite_tac [subst_eta] >> fs [] >>
+        rw[ALOOKUP_ZIP_MAP] )
+      )>>
     PairCases_on`p`>>
     match_mp_tac (transitive_po_of_spo |> SIMP_RULE std_ss [AND_IMP_INTRO] |> GEN_ALL)>>
     gvs[check_transitivity_def,check_ws_def]>>
@@ -2761,31 +2927,43 @@ Proof
     rw[]>>
     simp[GSYM LIST_TO_SET_MAP]>>
     rw[sat_implies_EL]>>
-    fs[MEM_COUNT_LIST]>>
-    pairarg_tac>>gs[]>>
+    fs[MEM_enumerate_iff]>>
+    pairarg_tac>>gs[PULL_EXISTS]>>
     first_x_assum drule>>
-    rw[]>>
-    drule_all lookup_extract_pids_r>>
-    simp[]>>
-    rw[]>>
-    drule extract_clauses_MEM_INR>>
-    disch_then drule>>
-    simp[EL_MAP]>>
-    rw[]>>
-    fs[EVERY_MEM]>>
-    first_x_assum drule>>
-    simp[]>>rw[]>>
-    drule unsatisfiable_not_sat_implies>>
-    simp[core_only_fml_build_fml,Abbr`fmll`] >>
-    once_rewrite_tac [subst_eta] >> fs [] >>
-    gvs [ALOOKUP_APPEND,ALOOKUP_ZIP_MAP] >>
-    qmatch_goalsub_abbrev_tac ‘subst f1’ >> strip_tac >>
-    qmatch_goalsub_abbrev_tac ‘subst f2’ >>
-    qsuff_tac ‘f1 = f2’ >-
-      (rw [] >> gvs []) >>
-    unabbrev_all_tac >>
-    fs [FUN_EQ_THM] >> rw [] >>
-    ntac 4 (CASE_TAC >> fs []) )
+    PURE_REWRITE_TAC[METIS_PROVE [] ``((P ⇒ Q) ⇒ R) ⇔ (~P ∨ Q) ⇒ R``]>>
+    strip_tac
+    >- (
+      rw[]>>
+      drule_all lookup_extract_pids_r>>
+      simp[]>>
+      rw[]>>
+      drule extract_clauses_MEM_INR>>
+      disch_then drule>>
+      simp[EL_MAP]>>
+      rw[]>>
+      fs[EVERY_MEM]>>
+      first_x_assum drule>>
+      simp[]>>rw[]>>
+      drule unsatisfiable_not_sat_implies>>
+      simp[core_only_fml_build_fml,Abbr`fmll`] >>
+      once_rewrite_tac [subst_eta] >> fs [] >>
+      gvs [ALOOKUP_APPEND,ALOOKUP_ZIP_MAP] >>
+      qmatch_goalsub_abbrev_tac ‘subst f1’ >> strip_tac >>
+      qmatch_goalsub_abbrev_tac ‘subst f2’ >>
+      qsuff_tac ‘f1 = f2’ >-
+        (rw [] >> gvs []) >>
+      unabbrev_all_tac >>
+      fs [FUN_EQ_THM] >> rw [] >>
+      ntac 4 (CASE_TAC >> fs []) )
+    >- (
+      gvs[EL_MAP]>>
+      match_mp_tac unsatisfiable_not_sat_implies>>
+      simp[]>>
+      drule check_contradiction_unsat>>
+      simp[unsatisfiable_def,satisfiable_def]>>
+      once_rewrite_tac [subst_eta] >> fs [] >>
+      rw[ALOOKUP_ZIP_MAP] )
+    )
   >- (
     (* Obj *)
     strip_tac>>
@@ -2855,20 +3033,40 @@ Proof
     disch_then(qspecl_then[`pfs`,`T`] mp_tac)>>simp[]>>
     strip_tac>>
     fs[EVERY_MEM,MEM_MAP,EXISTS_PROD]>>
-    gvs[change_obj_subgoals_def,MEM_COUNT_LIST,ADD1]>>
-    first_assum(qspec_then`0` mp_tac)>>
-    first_x_assum(qspec_then`1` mp_tac)>>
-    simp[]>>
-    strip_tac>> drule_all lookup_extract_pids_r>>
-    simp[]>> strip_tac>>
-    drule_all extract_clauses_MEM_INR>>
-    simp[]>> strip_tac>>
-    strip_tac>> drule_all lookup_extract_pids_r>>
-    simp[]>> strip_tac>>
-    drule_all extract_clauses_MEM_INR>>
-    simp[]>> strip_tac>>
-    res_tac >>fs[]>>
+    gvs[change_obj_subgoals_def,MEM_enumerate_iff,ADD1,PULL_EXISTS]>>
     qmatch_asmsub_rename_tac`model_bounding fnew fold`>>
+    `unsatisfiable (core_only_fml T fml ∪ {not (model_bounding fnew fold)})` by (
+      first_x_assum(qspec_then`0` mp_tac)>>
+      simp[]>>
+      PURE_REWRITE_TAC[METIS_PROVE [] ``((P ⇒ Q) ⇒ R) ⇔ (~P ∨ Q) ⇒ R``]>>
+      strip_tac
+      >- (
+        drule_all lookup_extract_pids_r>>
+        simp[]>> strip_tac>>
+        drule_all extract_clauses_MEM_INR>>
+        simp[]>>
+        strip_tac>>
+        first_x_assum drule>>simp[])
+      >- (
+        drule check_contradiction_unsat>>
+        simp[unsatisfiable_def,satisfiable_def]
+      ))>>
+    `unsatisfiable (core_only_fml T fml ∪ {not (model_bounding fold fnew)})` by (
+      first_x_assum(qspec_then`1` mp_tac)>>
+      simp[]>>
+      PURE_REWRITE_TAC[METIS_PROVE [] ``((P ⇒ Q) ⇒ R) ⇔ (~P ∨ Q) ⇒ R``]>>
+      strip_tac
+      >- (
+        drule_all lookup_extract_pids_r>>
+        simp[]>> strip_tac>>
+        drule_all extract_clauses_MEM_INR>>
+        simp[]>>
+        strip_tac>>
+        first_x_assum drule>>simp[])
+      >- (
+        drule check_contradiction_unsat>>
+        simp[unsatisfiable_def,satisfiable_def]
+      ))>>
     `∀w.
       satisfies w (core_only_fml T fml) ⇒
       eval_obj (SOME fold) w =
@@ -2899,7 +3097,8 @@ Proof
       metis_tac[])>>
     fs[valid_conf_def]>>
     rw[bimp_obj_def,imp_obj_def,sat_obj_le_def]>>
-    asm_exists_tac>>simp[])
+    first_x_assum drule>>
+    metis_tac[])
   >-
     (every_case_tac>>rw[])
 QED
